coq/handwritten/CryptolToCoq/SAWCoreBitvectors.v
@@ -11,6 +11,8 @@ From CryptolToCoq Require Import SAWCoreVectorsAsCoqVectors.
 
 Import SAWCorePrelude.
 
+Create HintDb SAWCoreBitvectors.
+
 
 (** Bitvector maximum and minimum values **)
 
@@ -34,22 +36,27 @@ Definition bvumin w : bitvector w := gen w _ (fun _ => false).
 Definition isBvsle w a b : Prop := bvsle w a b = true.
 Definition isBvsle_def w a b : bvsle w a b = true <-> isBvsle w a b := reflexivity _.
 Definition isBvsle_def_opp w a b : bvslt w a b = false <-> isBvsle w b a. Admitted.
+Hint Rewrite isBvsle_def isBvsle_def_opp : SAWCoreBitvectors.
 Instance PreOrder_isBvsle w : PreOrder (isBvsle w). Admitted.
 
 Definition isBvslt w a b : Prop := bvslt w a b = true.
 Definition isBvslt_def w a b : bvslt w a b = true <-> isBvslt w a b := reflexivity _.
 Definition isBvslt_def_opp w a b : bvsle w a b = false <-> isBvslt w b a. Admitted.
+Hint Rewrite isBvslt_def isBvslt_def_opp : SAWCoreBitvectors.
 Instance PreOrder_isBvslt w : PreOrder (isBvslt w). Admitted.
 
 Definition isBvule w a b : Prop := bvule w a b = true.
 Definition isBvule_def w a b : bvule w a b = true <-> isBvule w a b := reflexivity _.
 Definition isBvule_def_opp w a b : bvult w a b = false <-> isBvule w b a. Admitted.
+Hint Rewrite isBvule_def isBvule_def_opp : SAWCoreBitvectors.
 Instance PreOrder_isBvule w : PreOrder (isBvule w). Admitted.
 
 Definition isBvult w a b : Prop := bvult w a b = true.
 Definition isBvult_def w a b : bvult w a b = true <-> isBvult w a b := reflexivity _.
 Definition isBvult_def_opp w a b : bvule w a b = false <-> isBvult w b a. Admitted.
+Hint Rewrite isBvult_def isBvult_def_opp : SAWCoreBitvectors.
 Instance PreOrder_isBvult w : PreOrder (isBvult w). Admitted.
+
 
 (** Converting between bitvector inqualities **)
 
@@ -67,6 +74,7 @@ Definition isBvult_to_isBvslt_pos w a b : isBvsle w (bvLit w 0) a ->
                                           isBvsle w (bvLit w 0) b ->
                                           isBvult w a b -> isBvslt w a b.
 Admitted.
+
 
 (** Other lemmas about bitvector inequalities **)
 
@@ -86,9 +94,32 @@ Admitted.
 
 (** Lemmas about bitvector equality **)
 
-Lemma bvEq_wrapped_bool (b : bool)
-  : not (bvEq 1 (if b then bvLit 1 1 else bvLit 1 0) (bvLit 1 0)) = b.
-Proof. destruct b; reflexivity. Qed.
+Lemma bvEq_eq  w a b : bvEq w a b = true <-> a = b. Admitted.
+Lemma bvEq_neq w a b : bvEq w a b = false <-> a <> b. Admitted.
+Hint Rewrite bvEq_eq bvEq_neq : SAWCoreBitvectors.
+
+Lemma bv_eq_if_true (b : bool) : (if b then bvLit 1 1 else bvLit 1 0) = bvLit 1 1 <-> b = true.
+Proof. split; intro H; destruct b; reflexivity || inversion H. Qed.
+Lemma bv_eq_if_false (b : bool) : (if b then bvLit 1 1 else bvLit 1 0) = bvLit 1 0 <-> b = false.
+Proof. split; intro H; destruct b; reflexivity || inversion H. Qed.
+
+Hint Rewrite bv_eq_if_true bv_eq_if_false : SAWCoreBitvectors.
+
+Lemma bv_neq_if_true (b : bool) : (if b then bvLit 1 1 else bvLit 1 0) <> bvLit 1 1 <-> b = false.
+Proof.
+  split; intro H; destruct b; try reflexivity || inversion H.
+  - pose (H0 := H (reflexivity _)); inversion H0.
+  - intro H0; inversion H0.
+Qed.
+
+Lemma bv_neq_if_false (b : bool) : (if b then bvLit 1 1 else bvLit 1 0) <> bvLit 1 0 <-> b = true.
+Proof.
+  split; intro H; destruct b; try reflexivity || inversion H.
+  - pose (H0 := H (reflexivity _)); inversion H0.
+  - intro H0; inversion H0.
+Qed.
+
+Hint Rewrite bv_neq_if_true bv_neq_if_false : SAWCoreBitvectors.
 
 
 (** Lemmas about bitvector addition **)
@@ -97,3 +128,54 @@ Lemma bvAdd_id_l w a : bvAdd w (bvLit w 0) a = a. Admitted.
 Lemma bvAdd_id_r w a : bvAdd w a (bvLit w 0) = a. Admitted.
 Lemma bvAdd_comm w a b : bvAdd w a b = bvAdd w b a. Admitted.
 Lemma bvAdd_assoc w a b c : bvAdd w (bvAdd w a b) c = bvAdd w a (bvAdd w b c). Admitted.
+
+
+(** Other rewriting hints not directly imvolving bitvectors **)
+
+Lemma and_bool_eq_true_lemma (b c : bool) : and b c = true <-> (b = true) /\ (c = true).
+Proof.
+  split.
+  - destruct b, c; auto.
+  - intro; destruct H; destruct b, c; auto.
+Qed.
+
+Lemma and_bool_eq_false_lemma (b c : bool) : and b c = false <-> (b = false) \/ (c = false).
+Proof.
+  split.
+  - destruct b, c; auto.
+  - intro; destruct H; destruct b, c; auto.
+Qed.
+
+Hint Rewrite and_bool_eq_true_lemma and_bool_eq_false_lemma : SAWCoreBitvectors.
+
+Lemma or_bool_eq_true_lemma (b c : bool) : or b c = true <-> (b = true) \/ (c = true).
+Proof.
+  split.
+  - destruct b, c; auto.
+  - intro; destruct H; destruct b, c; auto.
+Qed.
+
+Lemma or_bool_eq_false_lemma (b c : bool) : or b c = false <-> (b = false) /\ (c = false).
+Proof.
+  split.
+  - destruct b, c; auto.
+  - intro; destruct H; destruct b, c; auto.
+Qed.
+
+Hint Rewrite or_bool_eq_true_lemma or_bool_eq_false_lemma : SAWCoreBitvectors.
+
+Lemma not_bool_eq_true_lemma (b : bool) : not b = true <-> b = false.
+Proof. split; destruct b; auto. Qed.
+
+Lemma not_bool_eq_false_lemma (b : bool) : not b = false <-> b = true.
+Proof. split; destruct b; auto. Qed.
+
+Hint Rewrite not_bool_eq_true_lemma not_bool_eq_false_lemma : SAWCoreBitvectors.
+
+Lemma sym_bool_true_eq_lemma (b : bool) : true = b <-> b = true.
+Proof. split; auto. Qed.
+
+Lemma sym_bool_false_eq_lemma (b : bool) : false = b <-> b = false.
+Proof. split; auto. Qed.
+
+Hint Rewrite sym_bool_true_eq_lemma sym_bool_false_eq_lemma : SAWCoreBitvectors.
